proof/correctproof/correct_check_mem_aux2.v
@@ -1,0 +1,927 @@
+From Coq Require Import List ZArith.
+Import ListNotations.
+From dx Require Import ResultMonad IR.
+From bpf.comm Require Import MemRegion Regs State Monad rBPFAST rBPFValues.
+From bpf.src Require Import DxNat DxIntegers DxValues DxMonad DxInstructions.
+
+From compcert Require Import Coqlib Values Clight Memory Integers.
+
+From bpf.clight Require Import interpreter.
+
+From bpf.proof Require Import MatchState Clightlogic clight_exec CommonLemma CorrectRel.
+
+From bpf.proof.correctproof Require Import correct_is_well_chunk_bool correct_get_sub correct_get_add correct_get_block_ptr correct_get_start_addr correct_get_block_size.
+
+Open Scope Z_scope.
+
+Section Check_mem_aux2.
+
+(** The program contains our function of interest [fn] *)
+Definition p : Clight.program := prog.
+
+(**r TODO: check_mem_aux2: memory_region -> perm -> addr -> chunk -> ptr *)
+
+(* [Args,Res] provides the mapping between the Coq and the C types *)
+Definition args  := [(memory_region:Type) ; (permission:Type); valu32_t; (AST.memory_chunk: Type)].
+Definition res  := valptr8_t.
+
+(* [f] is a Coq Monadic function with the right type *)
+Definition f := check_mem_aux2.
+
+(* [fn] is the Cligth function which has the same behaviour as [f] *)
+Definition fn: Clight.function := f_check_mem_aux2.
+
+Definition is_vlong (v: val) :=
+  match v with
+  | Vlong _ => True
+  | _       => False
+  end.
+
+Variable bl_region : block.
+
+Definition match_arg  :
+  DList.t (fun x => x -> val -> State.state -> Memory.Mem.mem -> Prop) args :=
+  DList.DCons
+    (my_match_region bl_region)
+    (DList.DCons
+        (stateless perm_correct)
+        (DList.DCons
+           (stateless valu32_correct)
+           (DList.DCons (stateless match_chunk)
+                        (DList.DNil _)))).
+
+Definition match_res (v1 :val) (v2:val) :=
+  v1 = v2 /\ ((exists b ofs, v1 = Vptr b ofs) \/ v1 = val32_zero).
+
+
+Ltac build_app_aux T :=
+  match T with
+  | ?F ?X => let ty := type of X in
+             let r := build_app_aux F in
+             constr:((mk ty X) :: r)
+  | ?X    => constr:(@nil dpair)
+  end.                                    
+
+Ltac get_function T :=
+  match T with
+  | ?F ?X => get_function F
+  | ?X    => X
+  end.
+
+Ltac build_app T :=
+  let a := build_app_aux T in
+  let v := (eval simpl in (DList.of_list_dp (List.rev a))) in
+  let f := get_function T in
+  match type of v with
+  | DList.t _ ?L =>
+      change T with (app (f: arrow_type L _) v)
+  end.
+
+Ltac change_app_for_body :=
+  match goal with
+  | |- @correct_body _ _ ?F _ _ _ _ _ _ _ _
+    => build_app F
+  end.
+
+Ltac change_app_for_statement :=
+  match goal with
+  | |- @correct_statement _ _ ?F _ _ _ _ _ _ _ _
+    => build_app F
+  end.
+
+Ltac prove_incl :=
+  simpl; unfold incl; simpl; intuition congruence.
+
+Ltac prove_in_inv :=
+  simpl; intuition subst; discriminate.
+
+Ltac correct_forward :=
+  match goal with
+  | |- @correct_body _ _ (bindM ?F1 ?F2)  _
+                     (Ssequence
+                        (Ssequence
+                           (Scall _ _ _)
+                           (Sset ?V ?T))
+                        ?R)
+                     _ _ _ _ _ _  =>
+      eapply correct_statement_seq_body_pure;
+      [ change_app_for_statement ;
+        let b := match T with
+                 | Ecast _ _ => constr:(true)
+                 | _         => constr:(false)
+                 end in
+        eapply correct_statement_call with (has_cast := b)
+      |]
+  | |- @correct_body _ _ (match  ?x with true => _ | false => _ end) _
+                     (Sifthenelse _ _ _)
+                     _ _ _ _ _ _  =>
+      eapply correct_statement_if_body; [prove_in_inv | destruct x ]
+  end.
+
+Lemma correct_function_check_mem_aux2_correct : forall a, correct_function3 p args res f fn (nil) true match_arg (stateless match_res) a.
+Proof.
+  correct_function_from_body args.
+  correct_body.
+  unfold f. unfold check_mem_aux2.
+  simpl.
+  (** goal: correct_body _ _ (bindM (is_well_chunk_bool ... *)
+  correct_forward.
+
+  my_reflex.
+  my_reflex.
+  reflexivity.
+  typeclasses eauto.
+
+  { unfold INV.
+    unfold var_inv_preserve.
+    intros.
+    unfold match_temp_env in *.
+    rewrite Forall_fold_right in *.
+    simpl in *.
+    intuition. clear - H2 H.
+    unfold match_elt in *;
+      unfold fst in *.
+    destruct (Maps.PTree.get _mr le);auto.
+    simpl in *.
+    destruct H2 ; split; auto.
+    unfold my_match_region in *.
+    all: destruct H; auto.
+  }
+
+  reflexivity.
+  reflexivity.
+  reflexivity.
+  prove_in_inv.
+  prove_in_inv.
+  reflexivity.
+  reflexivity.
+
+  intros.
+  change (match_temp_env INV le st m) in H.
+  unfold INV in H.
+  get_invariant _chunk.
+  exists (v::nil).
+  split.
+  unfold map_opt. unfold exec_expr. rewrite p0.
+  reflexivity.
+  intros. simpl.
+  tauto.
+
+  intros.
+  (** goal: correct_body _ _ (if x then ... *)
+  correct_forward. 2:{ (**r if-else branch *)
+  unfold correct_body.
+  intros.
+  unfold Monad.returnM, val32_zero.
+  unfold returnM.
+  unfold Monad.returnM.
+  intros.
+  exists (Vint Int.zero), m, Events.E0.
+  repeat split.
+
+  forward_star.
+  forward_star.
+  unfold Int.zero.
+  forward_star.
+  reflexivity.
+  intuition.
+  constructor.
+  reflexivity.
+  }
+  (**r if-then branch *)
+
+  (** goal: correct_body p val (bindM (get_block_ptr c) *)
+  eapply correct_statement_seq_body_pure.
+  change_app_for_statement.
+  eapply correct_statement_call with (has_cast := false).
+  my_reflex.
+  my_reflex.
+  reflexivity.
+  typeclasses eauto.
+  { unfold INV.
+    unfold var_inv_preserve.
+    intros.
+    unfold match_temp_env in *.
+    rewrite Forall_fold_right in *.
+    simpl in *.
+    destruct H; subst.
+    intuition.
+  }
+  reflexivity.
+  reflexivity.
+  reflexivity.
+  prove_in_inv.
+  prove_in_inv.
+  reflexivity.
+  reflexivity.
+
+
+  {
+    unfold INV; intro H.
+    correct_Forall.
+    get_invariant _mr.
+    exists (v::nil).
+    split.
+    unfold map_opt. unfold exec_expr. rewrite p0.
+    reflexivity.
+    intros. simpl.
+    intuition. eauto.
+  }
+  intros.
+  (** goal: correct_body _ _ (bindM (get_start_addr c) ... *)
+  eapply correct_statement_seq_body_pure.
+  change_app_for_statement.
+  eapply correct_statement_call with (has_cast := false).
+  my_reflex.
+  my_reflex.
+  reflexivity.
+  typeclasses eauto.
+  { unfold INV.
+    unfold var_inv_preserve.
+    intros.
+    unfold match_temp_env in *.
+    rewrite Forall_fold_right in *.
+    simpl in *.
+    destruct H; subst.
+    intuition.
+  }
+  reflexivity.
+  reflexivity.
+  reflexivity.
+  prove_in_inv.
+  prove_in_inv.
+  reflexivity.
+  reflexivity.
+  unfold INV; intro H.
+  correct_Forall.
+  get_invariant _mr.
+  exists (v::nil).
+  split.
+  unfold map_opt,exec_expr.
+  rewrite p0.
+  reflexivity.
+  simpl. intros.
+  intuition eauto.
+  intros.
+  (** goal: correct_body _ _ (bindM (get_block_size c) ... *)
+  eapply correct_statement_seq_body_pure.
+  change_app_for_statement.
+  eapply correct_statement_call with (has_cast := false).
+  my_reflex.
+  my_reflex.
+  reflexivity.
+  typeclasses eauto.
+  { unfold INV.
+    unfold var_inv_preserve.
+    intros.
+    unfold match_temp_env in *.
+    rewrite Forall_fold_right in *.
+    simpl in *.
+    destruct H; subst.
+    intuition.
+  }
+  reflexivity.
+  reflexivity.
+  reflexivity.
+  prove_in_inv.
+  prove_in_inv.
+  reflexivity.
+  reflexivity.
+
+  unfold INV; intro H.
+  correct_Forall.
+  get_invariant _mr.
+  (**  exists lval : list val, _ [Etempvar _mr3 _] = Some lval *)
+  exists (v::nil).
+  split.
+  unfold map_opt, exec_expr.
+  rewrite p0; reflexivity.
+  simpl;intros.
+  intuition eauto.
+  intros.
+  (** goal:  correct_body _ _ (bindM (get_sub c0 x0) ... *)
+  eapply correct_statement_seq_body_pure.
+  change_app_for_statement.
+  eapply correct_statement_call with (has_cast := false).
+  my_reflex.
+  my_reflex.
+  reflexivity.
+  typeclasses eauto.
+  { unfold INV.
+    unfold var_inv_preserve.
+    intros.
+    unfold match_temp_env in *.
+    rewrite Forall_fold_right in *.
+    simpl in *.
+    destruct H; subst.
+    intuition.
+  }
+  reflexivity.
+  reflexivity.
+  reflexivity.
+  prove_in_inv.
+  prove_in_inv.
+  reflexivity.
+  reflexivity.
+
+  unfold INV; intro H.
+  correct_Forall.
+  get_invariant _addr.
+  get_invariant _start.
+  (**  exists lval : list val, _ [(Etempvar _addr0 _); (Etempvar _start _)] = Some lval *)
+  exists ([v; v0]).
+  split.
+  unfold map_opt, exec_expr.
+  rewrite p0, p1; reflexivity.
+  simpl;intros.
+  intuition; eauto. (**r we lost the evident that `correct_get_start_addr.match_res x0 v0 st3 m3` *)
+  eauto. (**r we lost one very imporant information: the input/output constraints *)
+  intros.
+  (** goal:  correct_body _ _ (bindM (get_add x2 (memory_chunk_to_valu32 c1)) ... *)
+  eapply correct_statement_seq_body_pure.
+  change_app_for_statement.
+  eapply correct_statement_call with (has_cast := false).
+  my_reflex.
+  my_reflex.
+  reflexivity.
+  typeclasses eauto.
+  { unfold INV.
+    unfold var_inv_preserve.
+    intros.
+    unfold match_temp_env in *.
+    rewrite Forall_fold_right in *.
+    simpl in *.
+    destruct H; subst.
+    intuition.
+  }
+  reflexivity.
+  reflexivity.
+  reflexivity.
+  prove_in_inv.
+  prove_in_inv.
+  reflexivity.
+  reflexivity.
+
+  unfold INV; intro H.
+  correct_Forall.
+  get_invariant _lo_ofs.
+  get_invariant _chunk.
+  unfold map_opt, exec_expr.
+  rewrite p0, p1.
+  exists ([v; v0]).
+  split.
+  unfold map_opt, exec_expr. reflexivity.
+  simpl;intros.
+  intuition eauto.
+
+  unfold stateless, valu32_correct, memory_chunk_to_valu32, well_chunk_Z.
+  unfold stateless, match_chunk, memory_chunk_to_valu32, well_chunk_Z in H2.
+  intuition eauto.
+  intros.
+  (** goal: correct_body _ _ (if then else ... *)
+
+  destruct (match x2 with
+  | Vint n2 => negb (Int.ltu n2 int32_0)
+  | _ => false
+  end && compu_lt_32 x3 x1) eqn: Hcond1.
+  destruct (compu_le_32 x2 (memory_chunk_to_valu32_upbound c2) &&
+  match val32_modu x2 (memory_chunk_to_valu32 c2) with
+  | Vint n2 => Int.eq int32_0 n2
+  | _ => false
+  end) eqn: Hcond2.
+  (**r we have three goals: 
+    1. if-Hcond1-then-if-Hcond2-then
+    2. if-Hcond1-then-if-Hcond2-else
+    3. if-Hcond1-else
+    *)
+  3:{
+    unfold list_rel_arg,app;
+    match goal with
+    |- correct_body _ _ _ _ ?B _ ?INV
+                 _ _ _ _ =>
+      let I := fresh "INV" in
+      set (I := INV) ; simpl in I;
+      let B1 := eval simpl in B in
+        change B with B1
+    end.
+    unfold correct_body.
+    unfold returnM, val32_zero.
+    intros.
+
+    unfold INV0, INV in H.
+    get_invariant_more _hi_ofs.
+    get_invariant_more _lo_ofs.
+    get_invariant_more _size.
+    get_invariant_more _chunk.
+    get_invariant_more _ptr.
+    unfold correct_get_add.match_res, valu32_correct in H0.
+    destruct H0 as (H0_eq & (vi0 & Hvi0_eq)).
+    unfold correct_get_sub.match_res, valu32_correct in H2.
+    destruct H2 as (H2_eq & (vi2 & Hvi2_eq)).
+    unfold correct_get_block_size.match_res, valu32_correct in H4.
+    destruct H4 as (H4_eq & (vi4 & Hvi4_eq)).
+    unfold stateless, match_chunk, memory_chunk_to_valu32 in H6.
+    unfold correct_get_block_ptr.match_res, val_ptr_correct in H8.
+    destruct H8 as (H9_eq & (b & ofs & Hvi9_eq)).
+    subst.
+
+    exists (Vint Int.zero), m, Events.E0.
+    repeat split.
+
+    (**r we need the info given by Hcond1 *)
+    unfold int32_0 in Hcond1.
+    assert (Hfalse: Int.ltu vi2 Int.zero = false). {
+      unfold Int.ltu.
+      rewrite Int.unsigned_zero. (**r Check zlt. *)
+      destruct (zlt (Int.unsigned vi2) 0).
+      assert (Hge: (Int.unsigned vi2) >= 0). { apply Int_unsigned_ge_zero. }
+      lia.
+      reflexivity.
+    }
+    rewrite Hfalse in Hcond1.
+    unfold negb in Hcond1; simpl in Hcond1.
+
+
+    forward_star.
+    repeat forward_star.
+    forward_star.
+    repeat forward_star. (**r Search (_ && _ = false).*)
+
+    simpl.
+    fold Int.zero.
+    rewrite Hfalse; simpl.
+    reflexivity.
+
+    rewrite Int_eq_one_zero; simpl.
+    forward_star.
+    repeat forward_star.
+    simpl.
+    rewrite Hcond1.
+    reflexivity.
+
+    forward_star.
+    repeat forward_star.
+    forward_star.
+    repeat forward_star.
+    rewrite Maps.PTree.gss.
+    reflexivity.
+    rewrite Int.eq_true.
+    reflexivity.
+
+    forward_star.
+    repeat forward_star.
+    rewrite Int.eq_true; unfold negb.
+
+    forward_star.
+    forward_star.
+    reflexivity.
+    intuition.
+
+    constructor; reflexivity.
+  }
+
+  2:{ (**r 2. if-Hcond1-then-if-Hcond2-else *)
+    unfold list_rel_arg,app;
+    match goal with
+    |- correct_body _ _ _ _ ?B _ ?INV
+                 _ _ _ _ =>
+      let I := fresh "INV" in
+      set (I := INV) ; simpl in I;
+      let B1 := eval simpl in B in
+        change B with B1
+    end.
+    unfold correct_body.
+    unfold returnM, val32_zero.
+    intros.
+
+    unfold INV0, INV in H.
+    get_invariant_more _hi_ofs.
+    get_invariant_more _lo_ofs.
+    get_invariant_more _size.
+    get_invariant_more _chunk.
+    get_invariant_more _ptr.
+    unfold correct_get_add.match_res, valu32_correct in H0.
+    destruct H0 as (H0_eq & (vi0 & Hvi0_eq)).
+    unfold correct_get_sub.match_res, valu32_correct in H2.
+    destruct H2 as (H2_eq & (vi2 & Hvi2_eq)).
+    unfold correct_get_block_size.match_res, valu32_correct in H4.
+    destruct H4 as (H4_eq & (vi4 & Hvi4_eq)).
+    unfold stateless, match_chunk, memory_chunk_to_valu32 in H6.
+    unfold correct_get_block_ptr.match_res, val_ptr_correct in H8.
+    destruct H8 as (H9_eq & (b & ofs & Hvi9_eq)).
+    subst.
+
+    (**r we need the info given by Hcond1, Hcond2 *)
+    unfold int32_0 in Hcond1, Hcond1.
+    assert (Hfalse: Int.ltu vi2 Int.zero = false). {
+      unfold Int.ltu.
+      rewrite Int.unsigned_zero. (**r Check zlt. *)
+      destruct (zlt (Int.unsigned vi2) 0).
+      assert (Hge: (Int.unsigned vi2) >= 0). { apply Int_unsigned_ge_zero. }
+      lia.
+      reflexivity.
+    }
+    rewrite Hfalse in Hcond1.
+    unfold negb in Hcond1; simpl in Hcond1.
+    (**r after we need the info about Hcond2, I do it here*)
+
+    (**r we also need those info below *)
+    assert (Hneq1: _lo_ofs <> _t'9). {
+      unfold _lo_ofs, _t'9.
+      intro Hneq; inversion Hneq.
+    }
+    assert (Hneq2: _chunk <> _t'9). {
+      unfold _chunk, _t'9.
+      intro Hneq; inversion Hneq.
+    }
+    
+    assert (He: Int.modulus - 1 = 4294967295). {
+      unfold Int.modulus, Int.wordsize, Wordsize_32.wordsize; reflexivity.
+    }
+    assert (Hwell_chunk_unsigned: Int.unsigned (Int.repr (well_chunk_Z c2)) = well_chunk_Z c2). {
+      destruct c2; simpl; try (fold Int.zero; apply Int.unsigned_zero); try rewrite Int.unsigned_repr; try reflexivity; try rewrite Int_max_unsigned_eq64; try lia.
+    }
+
+    assert (Hchunk_ne_zero: Int.eq (Int.repr (well_chunk_Z c2)) Int.zero = false). {
+      unfold Int.zero.
+      destruct c2; unfold Int.eq; simpl;
+      repeat rewrite Int.unsigned_repr; try rewrite Int_max_unsigned_eq64; try apply zeq_false; try lia.
+    }
+
+    fold Int.zero Int.mone.
+    exists (Vint Int.zero), m, Events.E0.
+    repeat split.
+
+    unfold val32_modu, memory_chunk_to_valu32, Val.modu, int32_0 in Hcond2.
+    rewrite Hchunk_ne_zero in Hcond2.
+
+    destruct (compu_le_32 (Vint vi2) (memory_chunk_to_valu32_upbound c2)) eqn: Heq1.
+    (**r if lo_ofs <= 4294967295U - chunk then *)
+    (**r Search (true && _). *)
+    rewrite andb_true_l in Hcond2.
+    unfold compu_le_32, memory_chunk_to_valu32_upbound in Heq1.
+    rewrite Int_max_unsigned_eq64 in Heq1.
+
+    forward_star.
+    repeat forward_star.
+    forward_star.
+    repeat forward_star.
+    simpl.
+    rewrite Hfalse; reflexivity.
+    rewrite Int_eq_one_zero; unfold negb.
+    forward_star.
+    repeat forward_star.
+    simpl.
+    rewrite Hcond1; reflexivity.
+    forward_star.
+    repeat forward_star.
+    forward_star.
+    repeat forward_star.
+    rewrite Maps.PTree.gss.
+    rewrite Int_eq_one_zero; reflexivity.
+    reflexivity.
+    forward_star.
+    repeat forward_star.
+    rewrite Int_eq_one_zero; unfold negb.
+    forward_star.
+    forward_star.
+    forward_star.
+    rewrite Maps.PTree.gso.
+    rewrite p1; reflexivity.
+    assumption.
+    rewrite Maps.PTree.gso.
+    rewrite p3; reflexivity.
+    assumption.
+    reflexivity.
+    reflexivity.
+    simpl.
+    unfold Int.sub; rewrite Int.unsigned_mone.
+    rewrite He.
+
+    rewrite Hwell_chunk_unsigned.
+    rewrite Heq1.
+    reflexivity.
+
+    forward_star.
+    repeat forward_star.
+    rewrite Int_eq_one_zero; unfold negb.
+    repeat forward_star.
+    rewrite Maps.PTree.gso.
+    rewrite p1; reflexivity.
+    assumption.
+    rewrite Maps.PTree.gso.
+    rewrite p3; reflexivity.
+    assumption.
+    simpl.
+
+
+    Transparent Archi.ptr64.
+    unfold Cop.sem_mod, Cop.sem_binarith, Cop.sem_cast; simpl.
+
+    rewrite Hchunk_ne_zero.
+    reflexivity.
+
+    reflexivity.
+    simpl.
+    rewrite Hcond2.
+    reflexivity.
+
+    forward_star.
+    repeat forward_star.
+    forward_star.
+    repeat forward_star.
+    rewrite Maps.PTree.gss.
+    reflexivity.
+    reflexivity.
+    repeat rewrite Int.eq_true; unfold negb.
+    forward_star.
+    repeat forward_star.
+    forward_star.
+    reflexivity.
+
+    (**r if not lo_ofs <= 4294967295U - chunk then if 0U == lo_ofs % chunk then *)
+    unfold compu_le_32, memory_chunk_to_valu32_upbound in Heq1.
+    (**r Search (_ && _ = false).*)
+    forward_star.
+    repeat forward_star.
+    forward_star.
+    repeat forward_star.
+    simpl.
+
+    rewrite Hfalse; unfold negb.
+    reflexivity.
+
+    forward_star.
+    repeat forward_star.
+    rewrite Int_eq_one_zero; unfold negb.
+    forward_star.
+    repeat forward_star.
+    simpl.
+    rewrite Hcond1;
+    reflexivity.
+
+    forward_star.
+    repeat forward_star.
+    forward_star.
+    repeat forward_star.
+    rewrite Maps.PTree.gss.
+    reflexivity.
+    reflexivity.
+    repeat rewrite Int_eq_one_zero; unfold negb.
+
+    forward_star.
+    repeat forward_star.
+    forward_star.
+    repeat forward_star.
+    rewrite Maps.PTree.gso.
+    rewrite p1; reflexivity.
+    assumption.
+    rewrite Maps.PTree.gso.
+    rewrite p3; reflexivity.
+    assumption.
+    reflexivity.
+    reflexivity.
+    simpl.
+
+    fold Int.mone.
+    unfold Int.sub; rewrite Int.unsigned_mone.
+    rewrite He.
+
+    rewrite Hwell_chunk_unsigned.
+    rewrite Int_max_unsigned_eq64 in Heq1.
+    rewrite Heq1.
+    reflexivity.
+    rewrite Int.eq_true; unfold negb.
+
+    forward_star.
+    repeat forward_star.
+    forward_star.
+    repeat forward_star.
+    forward_star.
+    repeat forward_star.
+    rewrite Maps.PTree.gss.
+    reflexivity.
+    reflexivity.
+    rewrite Int.eq_true; unfold negb.
+    forward_star.
+    repeat forward_star.
+    forward_star.
+    reflexivity.
+    intuition.
+    constructor; reflexivity.
+  }
+  (**r goal: correct_body p val (bindM (get_block_perm c) ... *)
+  TODO.
+  unfold list_rel_arg,app;
+  match goal with
+  |- correct_body _ _ _ _ ?B _ ?INV
+               _ _ _ _ =>
+    let I := fresh "INV" in
+    set (I := INV) ; simpl in I;
+    let B1 := eval simpl in B in
+      change B with B1
+  end.
+  unfold correct_body.
+  intro.
+  destruct (returnM (Val.add x x2) st5) eqn: Hreturn; [idtac | constructor].
+  unfold returnM in Hreturn.
+  destruct p0.
+  intros.
+
+  (**r we need the value of those vairable in the memory, they will be used later *)
+  unfold INV0, INV in H.
+  get_invariant_more _hi_ofs.
+  get_invariant_more _lo_ofs.
+  get_invariant_more _size.
+  get_invariant_more _chunk.
+  get_invariant_more _ptr.
+  unfold correct_get_add.match_res, valu32_correct in H0.
+  destruct H0 as (H0_eq & (vi0 & Hvi0_eq)).
+  unfold correct_get_sub.match_res, valu32_correct in H2.
+  destruct H2 as (H2_eq & (vi2 & Hvi2_eq)).
+  unfold correct_get_block_size.match_res, valu32_correct in H4.
+  destruct H4 as (H4_eq & (vi4 & Hvi4_eq)).
+  unfold stateless, match_chunk, memory_chunk_to_valu32 in H6.
+  unfold correct_get_block_ptr.match_res, val_ptr_correct in H8.
+  destruct H8 as (H9_eq & (b & ofs & Hvi9_eq)).
+  subst.
+
+  exists (Val.add (Vptr b ofs) (Vint vi2)), m, Events.E0.
+  repeat split.
+  + 
+    Transparent Archi.ptr64.
+    forward_star.
+    repeat forward_star.
+    forward_star.
+    repeat forward_star.
+    unfold Cop.bool_val, Val.of_bool, Cop.sem_cmp, Cop.sem_binarith, Cop.sem_cast; simpl.
+    unfold Int.ltu.
+    fold Int.zero.
+    rewrite Int.unsigned_zero.
+    assert (Hvi3_ge: ((Int.unsigned vi2) >= 0)%Z). {
+      assert (Hhi_range: (0 <= Int.unsigned vi2 <= Int.max_unsigned)%Z).
+      apply Int.unsigned_range_2.
+      lia.
+    }
+    rewrite zlt_false; simpl.
+    rewrite Int_eq_one_zero; reflexivity.
+    assumption.
+
+    (** Smallstep.star _ _ (State _ (if negb false ... *)
+    simpl.
+    forward_star.
+    forward_star.
+    unfold Cop.sem_cast, Val.of_bool; simpl.
+    apply andb_prop in Hcond1.
+    destruct Hcond1 as (Hcond1_1 & Hcond1_2).
+    unfold compu_lt_32 in Hcond1_2.
+    rewrite Hcond1_2; simpl.
+    rewrite Int_eq_one_zero; reflexivity.
+    forward_star.
+    repeat forward_star.
+    forward_star.
+    repeat forward_star.
+    rewrite Maps.PTree.gss; reflexivity.
+    reflexivity.
+    (** Smallstep.star _ _(State _ (if negb (Int.eq Int.one Int.zero) then ... *)
+    forward_star.
+    rewrite Int_eq_one_zero.
+    unfold negb.
+    repeat forward_star.
+
+    (**r after we need the info about Hcond2, I do it here*)
+    apply andb_prop in Hcond2.
+    destruct Hcond2 as (Hcond2_1 & Hcond2_2).
+    unfold compu_le_32, memory_chunk_to_valu32_upbound in Hcond2_1.
+    rewrite Int_max_unsigned_eq64 in Hcond2_1.
+    unfold val32_modu, Val.modu, memory_chunk_to_valu32 in Hcond2_2.
+    
+    destruct (Int.eq (Int.repr (well_chunk_Z c1)) Int.zero) eqn: Heq_zero; try discriminate.
+
+    (**r we also need those info below *)
+    assert (Hneq1: _lo_ofs <> _t'8). {
+      unfold _lo_ofs, _t'8.
+      intro Hneq; inversion Hneq.
+    }
+    assert (Hneq2: _chunk <> _t'8). {
+      unfold _chunk, _t'8.
+      intro Hneq; inversion Hneq.
+    }
+
+    forward_star.
+    forward_star.
+    (**r the 1st place I need _lo_ofs & _chunk *)
+    apply Maps.PTree.gso with (x:=Vint Int.one) (m:=le5) in Hneq1.
+    rewrite Hneq1.
+    rewrite p1; reflexivity.
+    apply Maps.PTree.gso with (x:=Vint Int.one) (m:=le5) in Hneq2.
+    rewrite Hneq2.
+    rewrite p3; reflexivity.
+    reflexivity.
+    reflexivity.
+    unfold Cop.bool_val, Val.of_bool; simpl.
+
+    (**the first place I need Hcond2 *)
+    fold Int.mone.
+    unfold Int.sub; rewrite Int.unsigned_mone.
+    assert (He: Int.modulus - 1 = 4294967295). {
+      unfold Int.modulus, Int.wordsize, Wordsize_32.wordsize; reflexivity.
+    }
+    rewrite He.
+
+    assert (Hwell_chunk_unsigned: Int.unsigned (Int.repr (well_chunk_Z c1)) = well_chunk_Z c1). {
+      destruct c1; simpl; try (fold Int.zero; apply Int.unsigned_zero); try rewrite Int.unsigned_repr; try reflexivity; try rewrite Int_max_unsigned_eq64; try lia.
+    }
+    rewrite Hwell_chunk_unsigned.
+    rewrite Hcond2_1; simpl.
+    rewrite Int_eq_one_zero; unfold negb; reflexivity.
+    Search (if true then _ else _).
+    match goal with
+    | |- context[if true then ?X else ?Y] =>
+        change (if true then X else Y) with X
+    end.
+
+    forward_star.
+    forward_star.
+    (**r the 2nd place I need _lo_ofs & _chunk *)
+    apply Maps.PTree.gso with (x:=Vint Int.one) (m:=le5) in Hneq1.
+    rewrite Hneq1.
+    rewrite p1; reflexivity.
+    apply Maps.PTree.gso with (x:=Vint Int.one) (m:=le5) in Hneq2.
+    rewrite Hneq2.
+    rewrite p3; reflexivity.
+
+    unfold Cop.sem_binary_operation; simpl.
+    unfold Cop.sem_mod, Cop.sem_binarith; simpl.
+    (**r here we need to prove `modu`, i.e. (well_chunk_Z c1) <> 0, we should see the Hypothesis `Hcond2` *)
+    rewrite Heq_zero;
+    reflexivity.
+    reflexivity.
+
+    unfold Cop.bool_val, Val.of_bool; simpl.
+    unfold int32_0, Int.zero in Hcond2_2.
+    rewrite Hcond2_2.
+    reflexivity.
+
+    forward_star.
+    repeat forward_star.
+    forward_star.
+    repeat forward_star.
+    rewrite Maps.PTree.gss.
+    rewrite Int_eq_one_zero.
+    reflexivity.
+    reflexivity.
+
+    rewrite Int_eq_one_zero; unfold negb.
+    forward_star.
+    repeat forward_star.
+
+    assert (Hneq3: _ptr <> _t'7). {
+      unfold _ptr, _t'7.
+      intro Hneq; inversion Hneq.
+    }
+    assert (Hneq4: _ptr <> _t'8). {
+      unfold _ptr, _t'8.
+      intro Hneq; inversion Hneq.
+    }
+    apply Maps.PTree.gso with (x:=Vint Int.one) (m:=(Maps.PTree.set _t'8 (Vint Int.one) le5)) in Hneq3; rewrite Hneq3.
+    apply Maps.PTree.gso with (x:=Vint Int.one) (m:=le5) in Hneq4; rewrite Hneq4.
+    rewrite p4; reflexivity.
+
+    assert (Hneq3: _lo_ofs <> _t'7). {
+      unfold _lo_ofs, _t'7.
+      intro Hneq; inversion Hneq.
+    }
+    apply Maps.PTree.gso with (x:=Vint Int.one) (m:=(Maps.PTree.set _t'8 (Vint Int.one) le5)) in Hneq3; rewrite Hneq3.
+    apply Maps.PTree.gso with (x:=Vint Int.one) (m:=le5) in Hneq1; rewrite Hneq1.
+    rewrite p1; reflexivity.
+    unfold Cop.sem_binary_operation, Cop.sem_add, Cop.classify_add; simpl.
+    reflexivity.
+    reflexivity.
+
+    unfold Ptrofs.mul, Ptrofs.of_intu.
+    assert (Hofs_one: Ptrofs.unsigned (Ptrofs.repr 1) = 1). {
+      apply Ptrofs.unsigned_repr.
+      rewrite Ptrofs_max_unsigned_eq32.
+      lia.
+    }
+    rewrite Hofs_one.
+    rewrite Z.mul_1_l.
+    rewrite Ptrofs.repr_unsigned.
+    constructor.
+    reflexivity.
+  + inversion Hreturn.
+    reflexivity.
+  + inversion Hreturn.
+    left; exists b, (Ptrofs.add ofs (Ptrofs.of_int vi2)).
+    reflexivity.
+  + constructor.
+  + inversion Hreturn.
+    reflexivity.
+Qed.
+
+End Check_mem_aux2.
+
+Close Scope Z_scope.
+
+Existing Instance correct_function_check_mem_aux2_correct.
