proof/correctproof/correct_get_addr_ofs.v
@@ -37,8 +37,6 @@ Section Get_addr_ofs.
   (* [f] is a Coq Monadic function with the right type *)
   Definition f : arrow_type args (M res) := get_addr_ofs.
 
-  Variable state_block: block. (**r a block storing all rbpf state information? *)
-
   (* [fn] is the Cligth function which has the same behaviour as [f] *)
   Definition fn: Clight.function := f_get_addr_ofs.
 
