proof/correctproof/correct_get_opcode_alu64.v
@@ -4,7 +4,7 @@ From Coq Require Import List Lia ZArith.
 From compcert Require Import Integers Values Clight Memory.
 Import ListNotations.
 
-From bpf.proof Require Import Clightlogic MatchState CorrectRel CommonLemma.
+From bpf.proof Require Import Clightlogic MatchState CorrectRel CommonLemma CommonLemmaNat.
 
 From bpf.clight Require Import interpreter.
 
@@ -30,13 +30,15 @@ Section Get_opcode_alu64.
   Definition f : arrow_type args (M res) := get_opcode_alu64.
 
   Variable state_block: block. (**r a block storing all rbpf state information? *)
+  Variable mrs_block: block.
+  Variable ins_block: block.
 
   (* [fn] is the Cligth function which has the same behaviour as [f] *)
   Definition fn: Clight.function := f_get_opcode_alu64.
 
   (* [match_arg] relates the Coq arguments and the C arguments *)
   Definition match_arg_list : DList.t (fun x => x -> val -> State.state -> Memory.Mem.mem -> Prop) args :=
-    (DList.DCons (stateless nat8_correct)
+    (DList.DCons (stateless opcode_alu64_nat8_correct)
                 (DList.DNil _)).
 
   (* [match_res] relates the Coq result and the C result *)
@@ -52,7 +54,8 @@ Section Get_opcode_alu64.
     repeat intro.
     get_invariant_more _op.
 
-    unfold stateless, nat8_correct in H0.
+    unfold stateless, opcode_alu64_nat8_correct in H0.
+    destruct H0 as (H0 & Hland & Hge).
     subst.
 
     eexists. exists m, Events.E0.
@@ -63,19 +66,42 @@ Section Get_opcode_alu64.
     - simpl.
       (**r Search (Int.zero_ext).*)
       rewrite Int.zero_ext_idem;[idtac | lia].
-      unfold match_res, opcode_alu64_correct, byte_to_opcode_alu64.
-      match goal with
-      | |- (match ?X with | _ => _ end) =>
-          destruct X; try (eexists; reflexivity)
-      end. (**r here we must give a detailed relation between alu_opcode and Vint ... int8_correct *)
-      admit.
+      unfold match_res, opcode_alu64_correct.
+      rewrite byte_to_opcode_alu64_if_same.
+      unfold byte_to_opcode_alu64_if.
+      rewrite Int.zero_ext_and; [simpl | lia].
+      rewrite nat8_land_240_255_eq; [| apply Hge].
+
+Ltac simpl_if Ht :=
+  match goal with
+  | |- context [if ?X then _ else _] =>
+    destruct X eqn: Ht; [rewrite Nat.eqb_eq in Ht | rewrite Nat.eqb_neq in Ht]
+  end.
+
+Ltac simpl_alu_opcode Hop := simpl_if Hop; [rewrite Hop; reflexivity | ].
+
+      simpl_alu_opcode Hadd.
+      simpl_alu_opcode Hsub.
+      simpl_alu_opcode Hmul.
+      simpl_alu_opcode Hdiv.
+      simpl_alu_opcode Hor.
+      simpl_alu_opcode Hand.
+      simpl_alu_opcode Hlsh.
+      simpl_alu_opcode Hrsh.
+      simpl_if Hneg.
+      destruct (c =? 135)%nat eqn: Hc_eq; [rewrite Nat.eqb_eq in Hc_eq; rewrite Hc_eq; reflexivity | eexists; reflexivity].
+      simpl_alu_opcode Hmod.
+      simpl_alu_opcode Hxor.
+      simpl_alu_opcode Hmov.
+      simpl_alu_opcode Harsh.
+      eexists; reflexivity.
     - simpl.
       constructor.
       rewrite Int.zero_ext_idem;[idtac | lia].
       simpl.
       rewrite Int.zero_ext_idem;[idtac | lia].
       reflexivity.
-Admitted.
+Qed.
 
 End Get_opcode_alu64.
 
